Fighting normal forms of typed combinators, unsuccessfully. Added intrinsically typed combinators, but they aren't very useful.

Lambda/IntrinsicallyTypedCombinators.v
@@ -11,118 +11,61 @@ Inductive Ty : Type :=
 
 Notation "a → b" := (TArr a b) (at level 60, right associativity).
 
-Inductive Tm : Type :=
-    | K : Tm
-    | S : Tm
-    | App : Tm -> Tm -> Tm
-    | zero : Tm
-    | succ : Tm
-    | rec  : Tm.
+Inductive Tm : Ty -> Type :=
+    | K : forall {a b : Ty}, Tm (a → b → a)
+    | S : forall {a b c : Ty}, Tm ((a → b → c) → (a → b) → a → c)
+    | App : forall {a b : Ty}, Tm (a → b) -> Tm a -> Tm b
+    | zero : Tm TNat
+    | succ : Tm (TNat → TNat)
+    | rec  : forall {a : Ty}, Tm (a → (TNat → a → a) → TNat → a).
 
 Notation "M @ N" := (App M N) (at level 50, left associativity).
 
-Inductive hasType : Tm -> Ty -> Prop :=
-    | hasType_K :
-        forall a b : Ty, hasType K (a → b → a)
-    | hasType_S :
-        forall a b c : Ty,
-          hasType S ((a → b → c) → (a → b) → a → c)
-    | hasType_App :
-        forall (a b : Ty) (f x : Tm),
-          hasType f (a → b) -> hasType x a ->
-            hasType (App f x) b
-    | hasType_zero :
-        hasType zero TNat
-    | hasType_succ :
-        hasType succ (TNat → TNat)
-    | hasType_rec :
-        forall a : Ty,
-          hasType rec (a → (TNat → a → a) → TNat → a).
-
-Inductive red : Tm -> Tm -> Prop :=
+Inductive red : forall {A : Ty}, Tm A -> Tm A -> Prop :=
     | red_K :
-        forall x y : Tm,
-          red (K @ x @ y) x
+        forall {A B : Ty} (f : Tm (A → B → A)) (a : Tm A) (b : Tm B),
+          red (K @ a @ b) a
     | red_S :
-        forall x y z : Tm,
-          red (S @ x @ y @ z) (x @ z @ (y @ z))
+        forall {A B C : Ty} (f : Tm (A → B → C)) (g : Tm (A → B)) (a : Tm A),
+          red (S @ f @ g @ a) (f @ a @ (g @ a))
     | red_rec_zero :
-        forall z s : Tm,
+        forall {A : Ty} (z : Tm A) (s : Tm (TNat → A → A)),
           red (rec @ z @ s @ zero) z
     | red_rec_succ :
-        forall z s n : Tm,
+        forall {A : Ty} (z : Tm A) (s : Tm (TNat → A → A)) (n : Tm TNat),
           red (rec @ z @ s @ (succ @ n)) (s @ n @ (rec @ z @ s @ n))
     | red_AppL :
-        forall t1 t1' t2 : Tm,
-          red t1 t1' -> red (t1 @ t2) (t1' @ t2)
+        forall {A B : Ty} (f f' : Tm (A → B)) (a : Tm A),
+          red f f' -> red (f @ a) (f @ a)
     | red_AppR :
-        forall t1 t2 t2' : Tm,
-          red t2 t2' -> red (t1 @ t2) (t1 @ t2').
+        forall {A B : Ty} (f : Tm (A → B)) (a a' : Tm A),
+          red a a' -> red (f @ a) (f @ a').
 
 Notation "A ~> B" := (red A B) (at level 60).
 
-Hint Constructors Ty Tm hasType red rtc : core.
+Hint Constructors Ty Tm red rtc : core.
 
-Definition reds := rtc red.
+Definition reds {A : Ty} (t1 t2 : Tm A) : Prop := rtc (@red A) t1 t2.
 
-Hint Unfold reds : core.
+Notation "A ~> B" := (red A B) (at level 60).
 
-Infix "~>*" := reds (at level 50).
+Definition isNormal {A : Ty} (a : Tm A) : Prop :=
+  forall a' : Tm A, ~ a ~> a'.
 
-Definition isNormal (t : Tm) : Prop :=
-  forall t' : Tm, ~ red t t'.
-
-Inductive Nf : Tm -> Prop :=
-    | Nf_K0    : Nf K
-    | Nf_K1    : forall t : Tm, Nf t -> Nf (K @ t)
-    | Nf_S0    : Nf S
-    | Nf_S1    : forall t : Tm, Nf t -> Nf (S @ t)
-    | Nf_S2    : forall t1 t2 : Tm, Nf t1 -> Nf t2 -> Nf (S @ t1 @ t2)
+Inductive Nf : forall {A : Ty}, Tm A -> Prop :=
+    | Nf_K0    : forall {A B : Ty}, Nf (@K A B)
+    | Nf_K1    : forall {A B : Ty} (a : Tm A), Nf a -> Nf (@K A B @ a)
+    | Nf_S0    : forall {A B C : Ty}, Nf (@S A B C)
+    | Nf_S1    : forall {A B C : Ty} (f : Tm (A → B → C)), Nf f -> Nf (S @ f)
+    | Nf_S2    : forall {A B C : Ty} (f : Tm (A → B → C)) (g : Tm (A → B)), Nf f -> Nf g -> Nf (S @ f @ g)
     | Nf_zero  : Nf zero
     | Nf_succ0 : Nf succ
-    | Nf_succ1 : forall t : Tm, Nf t -> Nf (succ @ t)
-    | Nf_rec0  : Nf rec
-    | Nf_rec1  : forall t : Tm, Nf t -> Nf (rec @ t)
-    | Nf_rec2  : forall t1 t2 : Tm, Nf t1 -> Nf t2 -> Nf (rec @ t1 @ t2)
-    | Nf_Ne    : forall t : Tm, Ne t -> Nf t
+    | Nf_succ1 : forall n : Tm TNat, Nf n -> Nf (succ @ n)
+    | Nf_rec0  : forall {A : Ty}, Nf (@rec A)
+    | Nf_rec1  : forall {A : Ty} (z : Tm A), Nf z -> Nf (rec @ z)
+    | Nf_rec2  : forall {A : Ty} (z : Tm A) (s : Tm (TNat → A → A)), Nf z -> Nf s -> Nf (rec @ z @ s).
 
-with Ne : Tm -> Prop :=
-    | Ne_App : forall t1 t2 : Tm, Ne t1 -> Nf t2 -> Ne (t1 @ t2)
-    | Ne_rec : forall t1 t2 t3 : Tm, Nf t1 -> Nf t2 -> Ne t3 -> Ne (rec @ t1 @ t2 @ t3).
-
-Inductive Nf' : Tm -> Prop :=
-    | Nf'K0   : Nf' K
-    | Nf'K1   : forall t : Tm, Nf' t -> Nf' (K @ t)
-    | Nf'S0   : Nf' S
-    | Nf'S1   : forall t : Tm, Nf' t -> Nf' (S @ t)
-    | Nf'S2   : forall t1 t2 : Tm, Nf' t1 -> Nf' t2 -> Nf' (S @ t1 @ t2)
-    | Nf'rec0 : Nf' rec
-    | Nf'rec1 : forall t : Tm, Nf' t -> Nf' (rec @ t)
-    | Nf'rec2 : forall t1 t2 : Tm, Nf' t1 -> Nf' t2 -> Nf' (rec @ t1 @ t2)
-    | Nf'Ne'  : forall t : Tm, Ne' t -> Nf' t
-
-with      Ne' : Tm -> Prop :=
-    | Ne'zero : Ne' zero
-    | Ne'succ : Ne' succ
-    | Ne'App  : forall t1 t2 : Tm, Ne' t1 -> Nf' t2 -> Ne' (t1 @ t2).
-
-Inductive Nf3 : Tm -> Prop :=
-    | Nf3K1   : forall t : Tm, Nf3 t -> Nf3 (K @ t)
-    | Nf3S0   : Nf3 S
-    | Nf3S1   : forall t : Tm, Nf3 t -> Nf3 (S @ t)
-    | Nf3S2   : forall t1 t2 : Tm, Nf3 t1 -> Nf3 t2 -> Nf3 (S @ t1 @ t2)
-    | Nf3rec0 : Nf3 rec
-    | Nf3rec1 : forall t : Tm, Nf3 t -> Nf3 (rec @ t)
-    | Nf3rec2 : forall t1 t2 : Tm, Nf3 t1 -> Nf3 t2 -> Nf3 (rec @ t1 @ t2)
-    | Nf3Ne'  : forall t : Tm, Ne3 t -> Nf3 t
-
-     with Ne3 : Tm -> Prop :=
-    | Ne3K0   : Ne3 K
-    | Ne3zero : Ne3 zero
-    | Ne3succ : Ne3 succ
-    | Ne3App  : forall t1 t2 : Tm, Ne3 t1 -> Nf3 t2 -> Ne3 (t1 @ t2).
-
-Hint Constructors Nf Ne Nf' Ne' Nf3 Ne3 : core.
+Hint Constructors Nf : core.
 
 Ltac wut :=
 repeat match goal with
@@ -139,33 +82,23 @@ repeat match goal with
     | H : isNormal ?t, H' : red ?t _ |- _ => destruct (H _ H')
     | |- isNormal _ => do 2 intro
     | H : exists _, _   |- _ => decompose [ex and] H; clear H
-    | H : Ne ?x          |- _ => is_var x + inv H
-    | H : Ne' ?x          |- _ => is_var x + inv H
+(*     | H : Ne ?x          |- _ => is_var x + inv H *)
+(*     | H : Ne' ?x          |- _ => is_var x + inv H *)
     | _ => auto
 end.
 
-Fixpoint Nf_isNormal {t : Tm} (nf : Nf t) {struct nf} : isNormal t
-
-with     Ne_isNormal {t : Tm} (ne : Ne t) {struct ne} : isNormal t.
+Lemma Nf_isNormal :
+  forall {A : Ty} {a : Tm A},
+    Nf a -> isNormal a.
 Proof.
-  destruct nf.
+  unfold isNormal.
+  induction 1.
     wut.
-    red. do 2 intro. inv H.
-    1-11: wut; eapply Nf_isNormal;
-      repeat match goal with
-          | |- red _ _ => eauto
-      end; eauto.
-    apply Ne_isNormal. assumption.
-  destruct ne.
-    wut.
-      eapply Ne_isNormal; eauto.
-      eapply Nf_isNormal; eauto.
-    wut.
-      eapply Nf_isNormal. 2: eauto. eauto.
-      eapply Nf_isNormal. 2: eauto. eauto.
-      eapply Ne_isNormal. 2: eauto. eauto.
-Qed.
+    do 2 intro.
+    Require Import Equality. Print red. inv H0.
+Abort.
 
+(*
 Fixpoint Nf'_isNormal {t : Tm} (nf : Nf' t) {struct nf} : isNormal t
 
 with     Ne'_isNormal {t : Tm} (ne : Ne' t) {struct ne} : isNormal t.
@@ -246,8 +179,12 @@ Proof.
       inv H0.
       inv H0. inv H4.
         inv H. inv H3. inv H2.
-        inv H.
-Abort.
+        inv H. inv H5. inv H4.
+  inv H0; inv H3.
+    inv H1.
+    inv H1.
+    inv H. inv H4. inv H3; inv H0. inv H. inv H8. inv H8.
+    
   
 Lemma isNormal_Nf' :
   forall {t : Tm} {a : Ty}, hasType t a -> isNormal t -> Nf' t.
@@ -283,7 +220,37 @@ Proof.
                   inv H0.
                   inv H0.
                   inv H. inv H10. inv H8.
-                    inv H0.
+                    inv H0. inv H0. inv 
+
+ inv H2. inv H8; inv H.
+                exfalso. eapply H1. eauto.
+                
+
+
+
+
+    constructor; auto. apply IHhasType2. wut. eapply H1. eauto.
+    constructor; auto. apply IHhasType2. wut. eapply H1. eauto.
+    inv H2.
+      admit.
+      constructor.
+        constructor.
+      assert (Nf' (S @ x0)).
+        admit.
+        inv H.
+          repeat constructor. inv H6. econstructor. auto.
+      constructor. auto.
+        assert (Nf'
+        constructor; auto. apply IHhasType2. wut. eapply H1. eauto.
+    constructor; auto. apply IHhasType2. wut. eapply H1. eauto. constructor.
+  destruct f. all: cycle 3.
+    constructor; auto. apply IHt2. wut. eapply H. eauto.
+    constructor; auto. apply IHt2. wut. eapply H. eauto.
+    constructor; auto. apply IHt2. wut. eapply H. eauto.
+    constructor; auto. apply IHt2. wut. eapply H. eauto.
+    constructor; auto. apply IHt2. wut. eapply H. eauto.
+    destruct t1_1. all: cycle 3.
+      repeat constructor. constructor. auto.
 Abort.
 
 Definition hasNormal (t : Tm) : Prop :=
@@ -404,3 +371,4 @@ Restart.
     wut.
       red. exists t. wut.
 Abort.
+*)
